\subsection{1}

The following is a statement in \While:
$$y \= 1\; \while{\neg(x=1)}{(y \= y*x \; x \= x-1)}$$
It computes the factorial of the initial value bound to x (provided that it is positive), and the result will be the final value of y. Draw a graphical representation of the abstract syntax tree.\\
\begin{forest}
[$S$
 [$S$
     [$y$]
     [$\=$]
     [$a$ [$1$]]
 ]
 [;]
 [$S$
     [\textbf{while}]
     [$b$
         [$\neg$]
         [$b$
             [$a$ [$x$]]
             [$\eq$]
             [$a$ [$1$]]
         ]
     ]
     [\textbf{do}]
     [$S$
         [$S$
             [$y$]
             [$\=$]
             [$a$
                 [$a$ [$y$]]
                 [$*$]
                 [$a$ [$x$]]
             ]
         ]
         [;]
         [$S$
             [$x$]
             [$\=$]
             [$a$
                 [$a$ [$x$]]
                 [$-$]
                 [$a$ [$1$]]
             ]
         ]
     ]
 ]
]
\end{forest}
